move stack related operation into a separate file

Rustv/Rustv.thy
@@ -1,360 +1,17 @@
 theory Rustv
-  imports Simpl.Vcg
+  imports Simpl.Vcg Defs BorrowStack
 begin
 
-datatype rust_error = invalid_ref
-
-datatype pointer = ptr_val nat
-datatype tag = tag_val nat
-datatype val = int_val int
-record tagged_ref =
-  pointer :: pointer
-  tag :: tag
-
-fun the_ptr :: "pointer \<Rightarrow> nat" where
-  "the_ptr (ptr_val p) = p"
-
-fun the_tag :: "tag \<Rightarrow> nat" where
-  "the_tag (tag_val t) = t"
-
-datatype ref_kind = Unique | SharedReadWrite | SharedReadOnly
-type_synonym 'a stack = "'a list"
+abbreviation "collect_tags_stack == BorrowStack.collect_tags"
+abbreviation "pop_tags_stack == BorrowStack.pop_tags"
+abbreviation "writable_stack == BorrowStack.writable"
+abbreviation "reborrow_pop_stack == BorrowStack.reborrow_pop"
+abbreviation "reborrow_stack == BorrowStack.reborrow"
 
 record globals_ram =
   memory :: "val list"
   tags :: "(ref_kind * tag set) stack list"
   issued_tags :: "tag list"
-
-fun collect_tags_stack :: "(ref_kind * tag set) stack \<Rightarrow> tag set" where
-  "collect_tags_stack stack = \<Union>(set (map snd stack))"
-lemma collect_tags_stack_spec:
-  "t \<in> collect_tags_stack stack \<longleftrightarrow> (\<exists>entry \<in> set stack. t \<in> snd entry)"
-proof (induction stack)
-qed auto
-
-inductive wf_reborrow :: "(ref_kind * tag set) stack \<Rightarrow> bool" where
-  (* An allocation root is a Unique reference (Box) *)
-  BorrowRoot: "wf_reborrow [(Unique, {t})]" |
-
-  (* Reborrowing from a Unique reference *)
-  ReborrowUniqueUnique:
-    "\<lbrakk>wf_reborrow ((Unique, {t}) # tail); t' \<notin> insert t (collect_tags_stack tail)\<rbrakk>
- \<Longrightarrow> wf_reborrow ((Unique, {t'}) # (Unique, {t}) # tail)" |
-  ReborrowUniqueSRW:
-    "\<lbrakk>wf_reborrow ((Unique, {t}) # tail); t' \<notin> insert t (collect_tags_stack tail)\<rbrakk>
- \<Longrightarrow> wf_reborrow ((SharedReadWrite, {t'}) # (Unique, {t}) # tail)" |
-  ReborrowUniqueSRO:
-    "\<lbrakk>wf_reborrow ((Unique, {t}) # tail); t' \<notin> insert t (collect_tags_stack tail)\<rbrakk>
- \<Longrightarrow> wf_reborrow ((SharedReadOnly, {t'}) # (Unique, {t}) # tail)" |
-
-  (* Reborrowing from a SharedReadWrite *)
-  ReborrowSRWUnique:
-    "\<lbrakk>wf_reborrow ((SharedReadWrite, ts) # tail); t' \<notin> ts \<union> collect_tags_stack tail\<rbrakk>
- \<Longrightarrow> wf_reborrow ((Unique, {t'}) # (SharedReadWrite, ts) # tail)" |
-  ReborrowSRWSRW:
-    "\<lbrakk>wf_reborrow ((SharedReadWrite, ts) # tail); t \<notin> ts \<union> collect_tags_stack tail\<rbrakk>
- \<Longrightarrow> wf_reborrow ((SharedReadWrite, insert t ts) # tail)" |
-  ReborrowSRWSRO:
-    "\<lbrakk>wf_reborrow ((SharedReadWrite, ts) # tail); t' \<notin> ts \<union> collect_tags_stack tail\<rbrakk>
- \<Longrightarrow> wf_reborrow ((SharedReadOnly, {t'}) # (SharedReadWrite, ts) # tail)" |
-
-  (* Reborrowing from a SharedReadOnly gives only a shared reference *)
-  ReborrowSROSRO:
-    "\<lbrakk>wf_reborrow ((SharedReadOnly, ts) # tail); t \<notin> ts \<union> collect_tags_stack tail\<rbrakk>
- \<Longrightarrow> wf_reborrow ((SharedReadOnly, insert t ts) # tail)"
-
-inductive_cases wf_reborrow_elims: "wf_reborrow stack"
-
-lemma wf_reborrow_nonempty:
-  assumes "wf_reborrow stack"
-  shows "stack \<noteq> []"
-using assms proof (rule wf_reborrow_elims)
-qed auto
-
-lemma wf_reborrow_root: "wf_reborrow stack \<Longrightarrow> \<exists>t. last stack = (Unique, {t})"
-proof (induction rule: wf_reborrow.induct)
-qed auto
-
-lemma unique_ref_head:
-  assumes "wf_reborrow ((Unique, ts) # end)"
-  shows "\<exists>t. ts = {t}"
-using assms proof (rule wf_reborrow_elims)
-qed auto
-
-lemma unique_ref:
-  assumes
-    "wf_reborrow stack"
-    "(Unique, ts) \<in> set stack"
-  shows "\<exists>t. ts = {t}"
-using assms(1) assms(2) proof (induction rule: wf_reborrow.induct)
-qed auto
-
-lemma wf_reborrow_pop:
-  assumes
-    "wf_reborrow stack"
-    "stack = st1 # st2 # rest"
-  shows "wf_reborrow (st2 # rest)"
-using assms proof (induction arbitrary: st1 rule: wf_reborrow.induct)
-qed auto
-
-lemma wf_reborrow_pop':
-  fixes top rest
-  assumes
-    "wf_reborrow (top # rest)"
-    "rest \<noteq> []"
-  shows "wf_reborrow rest"
-using assms proof (induction "(top # rest)" arbitrary: top rule: wf_reborrow.induct)
-qed auto
-
-lemma shared_read_only_top:
-  assumes
-    "wf_reborrow stack"
-    "\<exists>entry \<in> set stack. fst entry = SharedReadOnly"
-  shows "fst (hd stack) = SharedReadOnly \<and> \<not>(\<exists>entry \<in> set (tl stack). fst entry = SharedReadOnly)"
-using assms proof (induction stack rule: wf_reborrow.induct)
-qed auto
-
-lemma wf_reborrow_top_tag_notin:
-  assumes
-    "wf_reborrow stack"
-    "target \<in> snd (hd stack)"
-  shows "target \<notin> collect_tags_stack (tl stack)"
-using assms proof (induction stack rule: wf_reborrow.induct)
-qed auto
-
-lemma wf_reborrow_tag_position_inj_zero:
-  assumes
-    "wf_reborrow stack"
-    "i < length stack"
-    "target \<in> snd (stack ! i)"
-    "target \<in> snd (stack ! 0)"
-  shows "i = 0"
-proof (cases i)
-  case 0
-  then show ?thesis by simp
-next
-  case (Suc i')
-  have "target \<in> snd (hd stack)" using assms wf_reborrow_nonempty
-    by (simp add: hd_conv_nth)
-  moreover have "target \<in> collect_tags_stack (tl stack)"
-    using assms collect_tags_stack_spec nth_tl wf_reborrow_nonempty
-    by (metis Nitpick.size_list_simp(2) Suc Suc_less_SucD nth_mem)
-  ultimately show ?thesis using wf_reborrow_top_tag_notin assms(1) by blast
-qed
-
-(* repetitive, obvious proof *)
-lemma wf_reborrow_tag_position_inj:
-  assumes
-    "wf_reborrow stack"
-    "i < length stack"
-    "j < length stack"
-    "target \<in> snd (stack ! i)"
-    "target \<in> snd (stack ! j)"
-  shows "i = j"
-using assms proof (induction stack arbitrary: i j rule: wf_reborrow.induct)
-  case (BorrowRoot t)
-  then show ?case by simp
-next
-  case (ReborrowUniqueUnique t tail t')
-  show ?case
-  proof (cases i)
-    case 0
-    then show ?thesis
-      using ReborrowUniqueUnique wf_reborrow.ReborrowUniqueUnique
-        wf_reborrow_tag_position_inj_zero by blast
-  next
-    case (Suc i')
-    note Suci = Suc
-    then show ?thesis
-    proof (cases j)
-      case 0
-      then show ?thesis
-        using ReborrowUniqueUnique wf_reborrow.ReborrowUniqueUnique
-          wf_reborrow_tag_position_inj_zero by blast
-    next
-      case (Suc j')
-      then show ?thesis using Suc Suci ReborrowUniqueUnique by auto
-    qed
-  qed
-next
-  case (ReborrowUniqueSRW t tail t')
-  then show ?case
-  proof (cases i)
-    case 0
-    then show ?thesis
-      using ReborrowUniqueSRW wf_reborrow.ReborrowUniqueSRW
-        wf_reborrow_tag_position_inj_zero by blast
-  next
-    case (Suc i')
-    note Suci = Suc
-    then show ?thesis
-    proof (cases j)
-      case 0
-      then show ?thesis
-        using ReborrowUniqueSRW wf_reborrow.ReborrowUniqueSRW
-          wf_reborrow_tag_position_inj_zero by blast
-    next
-      case (Suc j')
-      then show ?thesis using Suc Suci ReborrowUniqueSRW by auto
-    qed
-  qed
-next
-  case (ReborrowUniqueSRO t tail t')
-  then show ?case
-  proof (cases i)
-    case 0
-    then show ?thesis
-      using ReborrowUniqueSRO wf_reborrow.ReborrowUniqueSRO
-        wf_reborrow_tag_position_inj_zero by blast
-  next
-    case (Suc i')
-    note Suci = Suc
-    then show ?thesis
-    proof (cases j)
-      case 0
-      then show ?thesis
-      using ReborrowUniqueSRO wf_reborrow.ReborrowUniqueSRO
-        wf_reborrow_tag_position_inj_zero by blast
-    next
-      case (Suc j')
-      then show ?thesis using Suc Suci ReborrowUniqueSRO by auto
-    qed
-  qed
-next
-  case (ReborrowSRWUnique ts tail t')
-  then show ?case
-  proof (cases i)
-    case 0
-    then show ?thesis
-      using ReborrowSRWUnique wf_reborrow.ReborrowSRWUnique
-        wf_reborrow_tag_position_inj_zero by blast
-  next
-    case (Suc i')
-    note Suci = Suc
-    then show ?thesis
-    proof (cases j)
-      case 0
-      then show ?thesis
-      using ReborrowSRWUnique wf_reborrow.ReborrowSRWUnique
-        wf_reborrow_tag_position_inj_zero by blast
-    next
-      case (Suc j')
-      then show ?thesis using Suc Suci ReborrowSRWUnique by auto
-    qed
-  qed
-next
-  case (ReborrowSRWSRW ts tail t)
-  then show ?case
-  proof (cases i)
-    case 0
-    then show ?thesis
-      using ReborrowSRWSRW wf_reborrow.ReborrowSRWSRW
-        wf_reborrow_tag_position_inj_zero by blast
-  next
-    case (Suc i')
-    note Suci = Suc
-    then show ?thesis
-    proof (cases j)
-      case 0
-      then show ?thesis
-      using ReborrowSRWSRW wf_reborrow.ReborrowSRWSRW
-        wf_reborrow_tag_position_inj_zero by blast
-    next
-      case (Suc j')
-      then show ?thesis using Suc Suci ReborrowSRWSRW
-        by (metis length_Cons nth_Cons_Suc)
-    qed
-  qed
-next
-  case (ReborrowSRWSRO ts tail t')
-  then show ?case
-  proof (cases i)
-    case 0
-    then show ?thesis
-      using ReborrowSRWSRO wf_reborrow.ReborrowSRWSRO
-        wf_reborrow_tag_position_inj_zero by blast
-  next
-    case (Suc i')
-    note Suci = Suc
-    then show ?thesis
-    proof (cases j)
-      case 0
-      then show ?thesis
-      using ReborrowSRWSRO wf_reborrow.ReborrowSRWSRO
-        wf_reborrow_tag_position_inj_zero by blast
-    next
-      case (Suc j')
-      then show ?thesis using Suc Suci ReborrowSRWSRO by auto
-    qed
-  qed
-next
-  case (ReborrowSROSRO ts tail t)
-  then show ?case
-  proof (cases i)
-    case 0
-    then show ?thesis
-      using ReborrowSROSRO wf_reborrow.ReborrowSROSRO
-        wf_reborrow_tag_position_inj_zero by blast
-  next
-    case (Suc i')
-    note Suci = Suc
-    then show ?thesis
-    proof (cases j)
-      case 0
-      then show ?thesis
-      using ReborrowSROSRO wf_reborrow.ReborrowSROSRO
-        wf_reborrow_tag_position_inj_zero by blast
-    next
-      case (Suc j')
-      then show ?thesis using Suc Suci ReborrowSROSRO
-        by (metis length_Cons nth_Cons_Suc)
-    qed
-  qed
-qed
-
-lemma wf_reborrow_tag_position_unique':
-  assumes
-    "wf_reborrow stack"
-    "target \<in> collect_tags_stack stack"
-  shows "\<exists>i. (i < length stack \<and> target \<in> snd (stack ! i)) \<and>
-  (\<forall>j. j < length stack \<and> target \<in> snd (stack ! j) \<longrightarrow> j = i)"
-proof -
-  have "\<exists>i < length stack. target \<in> snd (stack ! i)"
-    using assms collect_tags_stack_spec by (metis in_set_conv_nth)
-  then obtain i where
-    "i < length stack"
-    "target \<in> snd (stack ! i)"
-    by auto
-  moreover
-  note calc = calculation
-  have "\<forall>j. j < length stack \<and> target \<in> snd (stack ! j) \<longrightarrow> j = i"
-  proof
-    fix j
-    show "j < length stack \<and> target \<in> snd (stack ! j) \<longrightarrow> j = i"
-    proof
-      assume "j < length stack \<and> target \<in> snd (stack ! j)"
-      then show "j = i" using calc assms wf_reborrow_tag_position_inj by auto
-    qed
-  qed
-  ultimately show "\<exists>i. (i < length stack \<and> target \<in> snd (stack ! i)) \<and>
-    (\<forall>j. j < length stack \<and> target \<in> snd (stack ! j) \<longrightarrow> j = i)"
-    by blast
-qed
-
-lemma wf_reborrow_tag_position_unique:
-  assumes
-    "wf_reborrow stack"
-    "target \<in> collect_tags_stack stack"
-  shows "\<exists>!i. i < length stack \<and> target \<in> snd (stack ! i)"
-  using wf_reborrow_tag_position_unique' assms by blast
-
-fun stack_finite :: "(ref_kind * tag set) stack \<Rightarrow> bool" where
-  "stack_finite [] = True" |
-  "stack_finite (s # stack) = (finite (snd s) \<and> stack_finite stack)"
-
-lemma stack_finite_spec: "stack_finite stack \<longleftrightarrow> (\<forall>s \<in> set stack. finite (snd s))"
-proof (induction stack)
-qed auto
 
 fun wf_tags :: "(ref_kind * tag set) stack list \<Rightarrow> bool" where
   "wf_tags [] = True" |
@@ -443,16 +100,6 @@ lemma collect_tags_last[simp, intro]:
 proof (induction ts)
 qed auto
 
-lemma collect_tags_stack_finite:
-  assumes "stack_finite stack"
-  shows "finite (collect_tags_stack stack)"
-  using assms stack_finite_spec by auto
-
-lemma stack_finite_finite_collect_tags_stack:
-  assumes "finite (collect_tags_stack stack)"
-  shows "stack_finite stack"
-  using assms by (simp add: stack_finite_spec)
-
 lemma collect_tags_finite[simp, intro]: "wf_tags ts \<Longrightarrow> finite (collect_tags ts)"
 proof (induction ts)
   case (Cons stack ts)
@@ -466,9 +113,6 @@ fun wf_heap :: "'a globals_ram_scheme \<Rightarrow> bool" where
     \<and> wf_tags (tags s)
     \<and> collect_tags (tags s) \<subseteq> set (issued_tags s)"
 
-fun pop_tags_stack :: "tag \<Rightarrow> (ref_kind * tag set) stack \<Rightarrow> (ref_kind * tag set) stack" where
-  "pop_tags_stack t stack = dropWhile (\<lambda>entry. t \<notin> snd entry) stack"
-
 fun pop_tags :: "tagged_ref \<Rightarrow> 'a globals_ram_scheme \<Rightarrow> 'a globals_ram_scheme" where
   "pop_tags r s =
     (let p = the_ptr (pointer r);
@@ -477,51 +121,6 @@ fun pop_tags :: "tagged_ref \<Rightarrow> 'a globals_ram_scheme \<Rightarrow> 'a
     s\<lparr> tags := (tags s)[p := stack'] \<rparr>)"
 
 fun_cases pop_tags_elims: "pop_tags r s = s'"
-
-lemma hd_dropWhile_stack:
-  assumes
-    "pop_tags_stack t stack = stack'"
-    "\<exists>entry \<in> set stack. t \<in> snd entry"
-  shows "t \<in> snd (hd stack')"
-  by (metis assms(1) assms(2) pop_tags_stack.simps dropWhile_eq_Nil_conv hd_dropWhile)
-
-lemma dropWhile_stack_reborrow:
-  "wf_reborrow stack \<and> dropWhile P stack \<noteq> [] \<Longrightarrow> wf_reborrow (dropWhile P stack)"
-proof (induction stack)
-  case Nil
-  then show ?case using wf_reborrow_nonempty by simp
-next
-  case (Cons top rest)
-  show ?case
-  proof (cases "P top")
-    case True
-    moreover have "dropWhile P rest \<noteq> []" using Cons.prems calculation by auto
-    moreover have "rest \<noteq> []" using calculation by auto
-    moreover have "wf_reborrow rest" using calculation Cons.prems wf_reborrow_pop' by auto
-    ultimately show ?thesis using Cons.IH by auto
-  next
-    case False
-    then show ?thesis using Cons.prems by simp
-  qed
-qed
-
-lemma dropWhile_stack_finite:
-  "stack_finite stack \<Longrightarrow> stack_finite (dropWhile P stack)"
-proof (induction stack)
-  case Nil
-  then show ?case by simp
-next
-  case (Cons st stack)
-  then have *: "stack_finite (dropWhile P stack)" by simp
-  then show ?case
-  proof (cases "P st")
-    case True
-    then show ?thesis using * by simp
-  next
-    case False
-    then show ?thesis using Cons.prems by simp
-  qed
-qed
 
 lemma pop_tags_wf_tags:
   assumes
@@ -643,53 +242,6 @@ proof -
   thus ?thesis using assms using collect_tags_spec' nth_mem by blast
 qed
 
-fun writable_stack :: "tag \<Rightarrow> (ref_kind * tag set) stack \<Rightarrow> bool" where
-  "writable_stack t [] \<longleftrightarrow> False" |
-  "writable_stack t ((k, ts) # stack) \<longleftrightarrow>
-    (if t \<in> ts then k = Unique \<or> k = SharedReadWrite else writable_stack t stack)"
-
-lemma writable_stack_in_collect_tags:
-  assumes "writable_stack t stack"
-  shows "t \<in> collect_tags_stack stack"
-using assms proof (induction stack)
-  case (Cons entry stack)
-  then show ?case using writable_stack.elims(2) by fastforce
-qed auto
-
-lemma writable_stack_the_index:
-  assumes
-    "wf_reborrow stack"
-    "writable_stack t stack"
-  shows "\<exists>!i. i < length stack \<and> t \<in> snd (stack ! i)"
-  using wf_reborrow_tag_position_unique writable_stack_in_collect_tags assms by simp
-
-lemma writable_stack_pop_tags_stack:
-  "writable_stack t stack \<Longrightarrow> writable_stack t (pop_tags_stack t stack)"
-proof (induction stack)
-  case Nil
-  then show ?case by simp
-next
-  case (Cons entry stack)
-  then show ?case using writable_stack.elims(2) by fastforce
-qed
-
-lemma writable_stack_pop_tags_stack':
-  assumes
-    "writable_stack t stack"
-    "pop_tags_stack t stack = stack'"
-  shows "(fst (hd stack') = Unique \<or> fst (hd stack') = SharedReadWrite)
-      \<and> t \<in> snd (hd stack')"
-    (is "?kind \<and> _")
-proof
-  show ?kind
-    using assms
-    by (metis hd_dropWhile list.collapse pop_tags_stack.elims prod.collapse writable_stack.simps(1)
-        writable_stack.simps(2) writable_stack_pop_tags_stack)
-next
-  show "t \<in> snd (hd stack')"
-    using hd_dropWhile_stack assms writable_stack_in_collect_tags by simp
-qed
-
 fun writable :: "tagged_ref \<Rightarrow> 'a globals_ram_scheme \<Rightarrow> bool" where
   "writable r s =
     (let p = the_ptr (pointer r) in
@@ -700,8 +252,8 @@ lemma writable_update[simp]: "writable r (memwrite r' v s) = writable r s"
   by simp
 
 lemma pop_tags_writable[intro]: "\<lbrakk>writable r s; wf_heap s\<rbrakk> \<Longrightarrow> writable r (pop_tags r s)"
-  apply (auto simp del: pop_tags_stack.simps)
-  by (metis nth_list_update_eq writable_stack_pop_tags_stack)
+  apply (auto simp del: BorrowStack.pop_tags.simps)
+  by (metis nth_list_update_eq writable_pop_tags)
 
 fun new_pointer :: "'a globals_ram_scheme \<Rightarrow> pointer" where
   "new_pointer s = ptr_val (length (memory s))"
@@ -725,326 +277,6 @@ lemma heap_new_wf_heap_update: "\<lbrakk>wf_heap s; heap_new v s = (r', s')\<rbr
   apply (erule heap_new_elims)
   by (auto simp add: Let_def wf_tags_snoc BorrowRoot)
 
-fun reborrow_stack :: "ref_kind \<Rightarrow> tag \<Rightarrow> (ref_kind * tag set) stack \<Rightarrow> (ref_kind * tag set) stack"
-  where
-  (* reborrwing Unique *)
-  "reborrow_stack Unique t ((Unique, ts) # stack) = (Unique, {t}) # (Unique, ts) # stack" |
-  "reborrow_stack Unique t ((SharedReadWrite, ts) # stack) =
-    (Unique, {t}) # (SharedReadWrite, ts) # stack" |
-  (* reborrowing SharedReadWrite *)
-  "reborrow_stack SharedReadWrite t ((Unique, ts) # stack) =
-    (SharedReadWrite, {t}) # (Unique, ts) # stack" |
-  "reborrow_stack SharedReadWrite t ((SharedReadWrite, ts) # stack) =
-    (SharedReadWrite, insert t ts) # stack" |
-  (* reborrwing SharedReadOnly *)
-  "reborrow_stack SharedReadOnly t ((Unique, ts) # stack) =
-    (SharedReadOnly, {t}) # (Unique, ts) # stack" |
-  "reborrow_stack SharedReadOnly t ((SharedReadWrite, ts) # stack) =
-    (SharedReadOnly, {t}) # (SharedReadWrite, ts) # stack" |
-  "reborrow_stack SharedReadOnly t ((SharedReadOnly, ts) # stack) =
-    (SharedReadOnly, insert t ts) # stack" |
-  (* other cases are uninteresting as reborrow is not well-formed *)
-  "reborrow_stack _ _ [] = []" |
-  "reborrow_stack Unique _ ((SharedReadOnly, _) # stack) = []" |
-  "reborrow_stack SharedReadWrite _ ((SharedReadOnly, _) # stack) = []"
-
-lemma reborrow_stack_hd:
-  assumes
-    "reborrow_stack r t stack = stack'"
-    "stack' \<noteq> []"
-  shows "r = fst (hd stack') \<and> t \<in> snd (hd stack')"
-using assms proof (cases rule: reborrow_stack.elims)
-qed auto
-
-fun_cases reborrow_stack_elims_Unique[case_names _ UniqueUnique UniqueSRW]:
-  "reborrow_stack Unique t stack = (Unique, ts) # stack'"
-fun_cases reborrow_stack_elims_SRW[case_names _ SRWUnique SRWSRW]:
-  "reborrow_stack SharedReadWrite t stack = (SharedReadWrite, ts) # stack'"
-fun_cases reborrow_stack_elims_SRO[case_names _ SROUnique SROSRW SROSRO]:
-  "reborrow_stack SharedReadOnly t stack = (SharedReadOnly, ts) # stack'"
-
-lemma wf_reborrow_reborrow_stack_Unique:
-  assumes
-    "wf_reborrow stack"
-    "t \<notin> collect_tags_stack stack"
-    "reborrow_stack Unique t stack = stack'"
-    "stack' \<noteq> []"
-  shows "wf_reborrow stack'"
-proof -
-  have p: "Unique = fst (hd stack') \<and> t \<in> snd (hd stack')"
-    using assms reborrow_stack_hd by simp
-  then obtain ts rest where
-    q: "stack' = (Unique, ts) # rest"
-    using assms by (metis list.collapse prod.collapse)
-  then have "wf_reborrow ((Unique, ts) # rest)"
-  proof (cases t stack ts rest rule: reborrow_stack_elims_Unique)
-    case _
-    then show ?case using assms(3) q by blast
-  next
-    case (UniqueUnique ts' stack)
-    moreover obtain t' where
-      "ts' = {t'}"
-      using assms(1) calculation(1) unique_ref_head by blast
-    moreover have "wf_reborrow ((Unique, {t}) # (Unique, {t'}) # stack)"
-    proof (rule ReborrowUniqueUnique)
-      show "wf_reborrow ((Unique, {t'}) # stack)"
-        using assms(1) calculation(1) calculation(4) by auto
-    next
-      have "t \<notin> {t'} \<union> collect_tags_stack stack"
-        using assms(2) calculation(1) calculation(4) by auto
-      then show "t \<notin> insert t' (collect_tags_stack stack)" by simp
-    qed
-    ultimately show ?thesis by simp
-  next
-    case (UniqueSRW ts' stack)
-    moreover have "wf_reborrow ((Unique, {t}) # (SharedReadWrite, ts') # stack)"
-    proof (rule ReborrowSRWUnique)
-      show "wf_reborrow ((SharedReadWrite, ts') # stack)"
-        using assms(1) calculation(1) by blast
-    next
-      show "t \<notin> ts' \<union> collect_tags_stack stack"
-        using assms(2) calculation(1) by auto
-    qed
-    ultimately show ?thesis by simp
-  qed
-  then show ?thesis by (simp add: q)
-qed
-
-lemma wf_reborrow_reborrow_stack_SRW:
-  assumes
-    "wf_reborrow stack"
-    "t \<notin> collect_tags_stack stack"
-    "reborrow_stack SharedReadWrite t stack = stack'"
-    "stack' \<noteq> []"
-  shows "wf_reborrow stack'"
-proof -
-  have p: "SharedReadWrite = fst (hd stack') \<and> t \<in> snd (hd stack')"
-    using assms reborrow_stack_hd by simp
-  then obtain ts rest where
-    q: "stack' = (SharedReadWrite, ts) # rest"
-    using assms by (metis list.collapse prod.collapse)
-  then have "wf_reborrow ((SharedReadWrite, ts) # rest)"
-  proof (cases t stack ts rest rule: reborrow_stack_elims_SRW)
-    case _
-    then show ?case using assms(3) q by blast
-  next
-    case (SRWUnique ts' stack)
-    moreover obtain t' where
-      "ts' = {t'}"
-      using assms(1) calculation(1) unique_ref_head by blast
-    moreover have "wf_reborrow ((SharedReadWrite, {t}) # (Unique, {t'}) # stack)"
-    proof (rule ReborrowUniqueSRW)
-      show "wf_reborrow ((Unique, {t'}) # stack)"
-        using assms SRWUnique calculation by simp
-    next
-      have "t \<notin> {t'} \<union> (collect_tags_stack stack)"
-        using assms(2) calculation(1) calculation(4) by auto
-      then show "t \<notin> insert t' (collect_tags_stack stack)" by auto
-    qed
-    moreover have "wf_reborrow ((SharedReadWrite, ts) # (Unique, ts') # stack)"
-      using calculation by simp
-    ultimately show ?thesis by simp
-  next
-    case (SRWSRW ts')
-    moreover have "wf_reborrow ((SharedReadWrite, insert t ts') # rest)"
-    proof (rule ReborrowSRWSRW)
-      show "wf_reborrow ((SharedReadWrite, ts') # rest)" using assms SRWSRW by simp
-    next
-      show "t \<notin> ts' \<union> collect_tags_stack rest" using assms SRWSRW by simp
-    qed
-    ultimately show ?thesis by simp
-  qed
-  then show ?thesis by (simp add: q)
-qed
-
-lemma wf_reborrow_reborrow_stack_SRO:
-  assumes
-    "wf_reborrow stack"
-    "t \<notin> collect_tags_stack stack"
-    "reborrow_stack SharedReadOnly t stack = stack'"
-    "stack' \<noteq> []"
-  shows "wf_reborrow stack'"
-proof -
-  have p: "SharedReadOnly = fst (hd stack') \<and> t \<in> snd (hd stack')"
-    using assms reborrow_stack_hd by simp
-  then obtain ts rest where
-    q: "stack' = (SharedReadOnly, ts) # rest"
-    using assms by (metis list.collapse prod.collapse)
-  then have "wf_reborrow ((SharedReadOnly, ts) # rest)"
-  proof (cases t stack ts rest rule: reborrow_stack_elims_SRO)
-    case _
-    then show ?case using assms(3) q by blast
-  next
-    case (SROUnique ts' stack)
-    moreover obtain t' where
-      "ts' = {t'}"
-      using assms(1) calculation(1) unique_ref_head by blast
-    moreover have "wf_reborrow ((SharedReadOnly, {t}) # (Unique, {t'}) # stack)"
-    proof (rule ReborrowUniqueSRO)
-      show "wf_reborrow ((Unique, {t'}) # stack)"
-        using assms calculation by simp
-    next
-      have "t \<notin> {t'} \<union> collect_tags_stack stack"
-        using assms(2) calculation(1) calculation(4) by auto
-      then show "t \<notin> insert t' (collect_tags_stack stack)" by simp
-    qed
-    ultimately show ?thesis by (simp add: q)
-  next
-    case (SROSRW ts' stack)
-    moreover have "wf_reborrow ((SharedReadOnly, {t}) # (SharedReadWrite, ts') # stack)"
-    proof (rule ReborrowSRWSRO)
-      show "wf_reborrow ((SharedReadWrite, ts') # stack)"
-        using assms(1) calculation(1) by auto
-    next
-      show "t \<notin> ts' \<union> collect_tags_stack stack"
-        using assms(2) calculation(1) by fastforce
-    qed
-    ultimately show ?thesis by (simp add: q)
-  next
-    case (SROSRO ts')
-    moreover have "wf_reborrow ((SharedReadOnly, insert t ts') # rest)"
-    proof (rule ReborrowSROSRO)
-      show "wf_reborrow ((SharedReadOnly, ts') # rest)"
-        using assms(1) calculation(1) by blast
-    next
-      show "t \<notin> ts' \<union> collect_tags_stack rest" using assms SROSRO by simp
-    qed
-    ultimately show ?thesis by simp
-  qed
-  then show ?thesis by (simp add: q)
-qed
-
-lemma wf_reborrow_reborrow_stack:
-  assumes
-    "wf_reborrow stack"
-    "t \<notin> collect_tags_stack stack"
-    "reborrow_stack k t stack = stack'"
-    "stack' \<noteq> []"
-  shows "wf_reborrow stack'"
-proof (cases k)
-  case Unique
-  then show ?thesis using assms wf_reborrow_reborrow_stack_Unique by simp
-next
-  case SharedReadWrite
-  then show ?thesis using assms wf_reborrow_reborrow_stack_SRW by simp
-next
-  case SharedReadOnly
-  then show ?thesis using assms wf_reborrow_reborrow_stack_SRO by simp
-qed
-
-lemma collect_tags_reborrow_stack_subset:
-  assumes "reborrow_stack k t stack = stack'"
-  shows "collect_tags_stack stack' \<subseteq> {t} \<union> collect_tags_stack stack"
-using assms proof(cases rule: reborrow_stack.elims)
-qed auto
-
-lemma stack_finite_reborrow_stack:
-  assumes
-    "reborrow_stack k t stack = stack'"
-    "stack_finite stack"
-  shows "stack_finite stack'"
-using assms collect_tags_reborrow_stack_subset stack_finite_finite_collect_tags_stack
-  by (meson collect_tags_stack_finite finite.emptyI finite.insertI finite_Un finite_subset)
-
-lemma notin_pop_tags_stack:
-  assumes "pop_tags_stack t stack = stack'"
-  shows "collect_tags_stack stack' \<subseteq> collect_tags_stack stack"
-using assms proof (induction stack arbitrary: stack')
-  case Nil
-  then show ?case by simp
-next
-  case (Cons entry stack)
-  show ?case
-  proof (cases "t \<in> snd entry")
-    case True
-    then have "stack' = entry # stack" using Cons.prems by simp
-    then show ?thesis by simp
-  next
-    case False
-    then have "stack' = pop_tags_stack t stack" using Cons.prems by simp
-    then show ?thesis using Cons.IH by auto
-  qed
-qed
-
-lemma wf_reborrow_stack_reborrow:
-  assumes
-    "wf_reborrow stack"
-    "writable_stack old stack"
-    "pop_tags_stack old stack = popped"
-    "reborrow_stack k new popped = stack'"
-    "new \<notin> collect_tags_stack stack"
-  shows "wf_reborrow stack'"
-proof -
-  have p: "wf_reborrow popped"
-    using assms
-    by (metis dropWhile_stack_reborrow pop_tags_stack.elims
-        writable_stack.simps(1) writable_stack_pop_tags_stack)
-  have q: "new \<notin> collect_tags_stack popped"
-    using assms notin_pop_tags_stack by fastforce
-  have "(fst (hd popped) = Unique \<and> old \<in> snd (hd popped))
-      \<or> (fst (hd popped) = SharedReadWrite \<and> old \<in> snd (hd popped))"
-    using assms writable_stack_pop_tags_stack' by blast
-  then show ?thesis
-  proof
-    assume "fst (hd popped) = Unique \<and> old \<in> snd (hd popped)"
-    then obtain ts rest where
-      "popped = (Unique, ts) # rest"
-      "old \<in> ts"
-      by (metis assms(2) assms(3) list.collapse prod.collapse
-          writable_stack.simps(1) writable_stack_pop_tags_stack)
-    moreover have "ts = {old}" using calculation assms p unique_ref_head by fastforce
-    moreover have "reborrow_stack k new ((Unique, {old}) # rest) = stack'"
-      using assms calculation by simp
-    then show ?thesis
-    proof (rule reborrow_stack.elims, auto)
-      show "wf_reborrow ((Unique, {new}) # (Unique, {old}) # rest)"
-        using assms calculation p q ReborrowUniqueUnique by simp
-    next
-      show "wf_reborrow ((SharedReadWrite, {new}) # (Unique, {old}) # rest)"
-        using assms calculation p q ReborrowUniqueSRW by simp
-    next
-      show "wf_reborrow ((SharedReadOnly, {new}) # (Unique, {old}) # rest)"
-        using assms calculation p q ReborrowUniqueSRO by simp
-    qed
-  next
-    assume "fst (hd popped) = SharedReadWrite \<and> old \<in> snd (hd popped)"
-    then obtain ts rest where
-      "popped = (SharedReadWrite, ts) # rest"
-      "old \<in> ts"
-      by (metis assms(2) assms(3) list.collapse prod.collapse
-          writable_stack.simps(1) writable_stack_pop_tags_stack)
-    moreover have "reborrow_stack k new ((SharedReadWrite, ts) # rest) = stack'"
-      using assms calculation by simp
-    then show ?thesis
-    proof (rule reborrow_stack.elims, auto)
-      show "wf_reborrow ((Unique, {new}) # (SharedReadWrite, ts) # rest)"
-        using assms calculation p q ReborrowSRWUnique by simp
-    next
-      show "wf_reborrow ((SharedReadWrite, insert new ts) # rest)"
-        using assms calculation p q ReborrowSRWSRW by simp
-    next
-      show "wf_reborrow ((SharedReadOnly, {new}) # (SharedReadWrite, ts) # rest)"
-        using assms calculation p q ReborrowSRWSRO by simp
-    qed
-  qed
-qed
-
-fun reborrow_pop_stack :: "ref_kind \<Rightarrow> tag \<Rightarrow> tag \<Rightarrow> (ref_kind * tag set) stack \<Rightarrow> (ref_kind * tag set) stack" where
-  "reborrow_pop_stack k child parent stack =
-    reborrow_stack k child (pop_tags_stack parent stack)"
-
-lemma reborrow_pop_stack_subset:
-  "collect_tags_stack (reborrow_pop_stack k child parent stack) \<subseteq> {child} \<union> collect_tags_stack stack"
-proof (induction stack arbitrary: child parent)
-  case Nil
-  then show ?case by simp
-next
-  case (Cons entry stack)
-  then show ?case
-    by (metis collect_tags_reborrow_stack_subset insert_is_Un insert_mono
-        notin_pop_tags_stack reborrow_pop_stack.elims subset_trans)
-qed
-
 fun reborrow :: "ref_kind \<Rightarrow> tagged_ref \<Rightarrow> 'a globals_ram_scheme \<Rightarrow> tagged_ref * 'a globals_ram_scheme" where
   "reborrow k r s =
     (let p = the_ptr (pointer r) in
@@ -1052,9 +284,9 @@ fun reborrow :: "ref_kind \<Rightarrow> tagged_ref \<Rightarrow> 'a globals_ram_
     let tags = (tags s)[p := reborrow_pop_stack k t (tag r) ((tags s) ! p)] in
     (\<lparr> pointer = pointer r, tag = t \<rparr>,  s\<lparr> tags := tags, issued_tags := t # issued_tags s \<rparr>))"
 
-declare reborrow_pop_stack.simps [simp del]
+declare BorrowStack.reborrow_pop.simps [simp del]
 fun_cases reborrow_elims: "reborrow k r s = (r', s')"
-declare reborrow_pop_stack.simps [simp]
+declare BorrowStack.reborrow_pop.simps [simp]
 
 lemma collect_tags_stack_reborrow_subset:
   assumes
@@ -1063,157 +295,65 @@ lemma collect_tags_stack_reborrow_subset:
   shows "collect_tags_stack stack' \<subseteq> {child} \<union> collect_tags_stack stack"
 proof -
   have "collect_tags_stack stack' \<subseteq> {child} \<union> collect_tags_stack popped"
-    using collect_tags_reborrow_stack_subset assms by simp
+    using collect_tags_reborrow_subset assms by simp
   moreover have "collect_tags_stack popped \<subseteq> collect_tags_stack stack"
-    using notin_pop_tags_stack assms by simp
+    using notin_pop_tags assms by simp
   ultimately show ?thesis by auto
 qed
 
 lemma collect_tags_reborrow_subset:
   "\<lbrakk>the_ptr (pointer r) < length (tags s); reborrow k r s = (r', s')\<rbrakk> \<Longrightarrow> collect_tags (tags s') \<subseteq> {new_tag s} \<union> collect_tags (tags s)"
   apply (erule reborrow_elims)
-  apply (simp add: Let_def del: reborrow_pop_stack.simps)
-  using collect_tags_update_subset reborrow_pop_stack_subset collect_tags_spec' nth_mem by blast
+  apply (simp add: Let_def del: reborrow_pop.simps)
+  using collect_tags_update_subset reborrow_pop_subset collect_tags_spec' nth_mem by blast
+
+lemma collect_tags_reborrow_subset':
+  "\<lbrakk>the_ptr (pointer r) < length (tags s)\<rbrakk> 
+  \<Longrightarrow> collect_tags (tags (snd (reborrow k r s))) \<subseteq> {new_tag s} \<union> collect_tags (tags s)"
+  apply (simp add: Let_def del: reborrow_pop.simps)
+  using collect_tags_update_subset reborrow_pop_subset collect_tags_spec' nth_mem by blast
 
 lemma reborrow_pointer: "reborrow k r s = (r', s') \<Longrightarrow> pointer r' = pointer r"
   apply (erule reborrow_elims)
-  by (auto simp: Let_def)
+  by (auto simp add: Let_def)
+
+lemma new_tag_collect:
+  assumes
+    "p < length ts"
+    "x \<in> collect_tags (ts[p := reborrow_pop_stack k t' t (ts ! p)])"
+      (is "x \<in> collect_tags (ts[p := ?stack])")
+    "collect_tags ts \<subseteq> issued"
+    "x \<notin> issued"
+  shows "x = t'"
+proof -
+  have "x \<in> collect_tags_stack ?stack \<union> collect_tags ts"
+    using assms collect_tags_update by blast
+  then have "x \<in> {t'} \<union> collect_tags_stack (ts ! p) \<union> collect_tags ts"
+    using reborrow_pop_subset by blast
+  moreover have "collect_tags_stack (ts ! p) \<subseteq> collect_tags ts"
+    using assms collect_tags_spec' nth_mem by blast
+  ultimately have "x \<in> {t'} \<union> collect_tags ts" by auto
+  then show ?thesis using assms by auto
+qed
+
+lemma reborrow_update_heap': "\<lbrakk>wf_heap s; writable r s\<rbrakk> \<Longrightarrow> wf_heap (snd (reborrow k r s))"
+  apply (auto simp add: Let_def)
+   apply (rule wf_tags_update, auto)
+    apply (rule wf_reborrow_reborrow_pop, auto)
+     apply (simp add: wf_tags_spec)
+  using new_tag_notin_at apply fastforce
+   apply (rule stack_finite_reborrow, auto)
+   apply (rule dropWhile_stack_finite)
+   apply (simp add: wf_tags_spec)
+  using new_tag_collect by auto
 
 lemma reborrow_update_heap: "\<lbrakk>wf_heap s; writable r s; reborrow k r s = (r', s')\<rbrakk> \<Longrightarrow> wf_heap s'"
-  apply (erule reborrow_elims)
-  apply auto
-    apply (simp add: Let_def) (* length condition is solved by simp *)
-   (* finite condition *)
-   apply (simp add: Let_def)
-   apply (rule wf_tags_update)
-     apply simp
-    prefer 2
-  using stack_finite_reborrow_stack wf_tags_spec apply (simp add: dropWhile_stack_finite)
-   apply (rule wf_reborrow_stack_reborrow, auto)
-  using nth_mem wf_tags_spec apply blast
-  using new_tag_notin_at apply fastforce
-  apply (subgoal_tac "collect_tags (tags s') \<subseteq> {new_tag s} \<union> collect_tags (tags s)")
-   apply (simp add: Let_def)
-   apply auto[1]
-  using collect_tags_reborrow_subset
-  by (metis new_tag.simps pop_tags_stack.elims reborrow.simps reborrow_pop_stack.simps)
-
-lemma decomp_pop_tags_stack_writable:
-  assumes
-    "writable_stack t stack"
-    "pop_tags_stack t stack = stack'"
-    "wf_reborrow stack"
-  shows "(\<exists>rest. stack' = (Unique, {t}) # rest)
-  \<or> (\<exists>rest ts. stack' = (SharedReadWrite, ts) # rest \<and> t \<in> ts)"
-using assms proof (induction stack)
-  case Nil
-  then show ?case by simp
-next
-  case (Cons entry stack)
-  then show ?case
-  proof (cases "t \<in> snd entry")
-    case True
-    moreover have "stack' = entry # stack" using Cons.prems calculation by simp
-    moreover have "fst entry = Unique \<or> fst entry = SharedReadWrite"
-      using Cons.prems(1) Cons.prems(2) calculation(2) writable_stack_pop_tags_stack' by fastforce
-    moreover have "entry = (Unique, {t}) \<or> (\<exists>ts. entry = (SharedReadWrite, ts) \<and> t \<in> ts)"
-      using Cons calculation
-      by (metis empty_iff insert_iff prod.collapse unique_ref_head)
-    ultimately show ?thesis by simp
-  next
-    case False
-    moreover have "writable_stack t stack" using Cons.prems calculation
-      by (metis eq_snd_iff list.inject writable_stack.elims(2))
-    moreover have "pop_tags_stack t stack = stack'" using Cons.prems calculation by simp
-    moreover have "wf_reborrow stack"
-      using Cons.prems wf_reborrow_pop' calculation(2) writable_stack.simps(1) by blast
-    ultimately show ?thesis using Cons.IH by simp
-  qed
-qed
-
-lemma decomp_reborrow_pop_stack_writable:
-  assumes
-    "writable_stack t stack"
-    "reborrow_pop_stack k t' t stack = stack'"
-    "wf_reborrow stack"
-    "t' \<notin> collect_tags_stack stack"
-  shows "
-  (\<exists>rest. k = Unique \<and> stack' = (Unique, {t'}) # (Unique, {t}) # rest)
-  \<or> (\<exists>rest. k = SharedReadWrite \<and> stack' = (SharedReadWrite, {t'}) # (Unique, {t}) # rest)
-  \<or> (\<exists>rest. k = SharedReadOnly \<and> stack' = (SharedReadOnly, {t'}) # (Unique, {t}) # rest)
-  \<or> (\<exists>rest ts. k = Unique \<and>  stack' = (Unique, {t'}) # (SharedReadWrite, ts) # rest \<and> t \<in> ts)
-  \<or> (\<exists>rest ts. k = SharedReadWrite \<and> stack' = (SharedReadWrite, insert t' ts) # rest \<and> t \<in> ts)
-  \<or> (\<exists>rest ts. k = SharedReadOnly \<and> stack' = (SharedReadOnly, {t'}) # (SharedReadWrite, ts) # rest \<and> t \<in> ts)"
-proof -
-  have *: "reborrow_stack k t' (pop_tags_stack t stack) = stack'" (is "reborrow_stack _ _ ?popped = _")
-    using assms by simp
-  then have "(\<exists>rest. ?popped = (Unique, {t}) # rest)
-  \<or> (\<exists>rest ts. ?popped = (SharedReadWrite, ts) # rest \<and> t \<in> ts)"
-    using assms decomp_pop_tags_stack_writable by simp
-  then show ?thesis
-  proof
-    assume "\<exists>rest. ?popped = (Unique, {t}) # rest"
-    then show ?thesis
-      using assms
-      by (metis (full_types) "*" reborrow_stack.simps(1) reborrow_stack.simps(3)
-          reborrow_stack.simps(5) ref_kind.exhaust)
-  next
-    assume "\<exists>rest ts. ?popped = (SharedReadWrite, ts) # rest \<and> t \<in> ts"
-    then show ?thesis
-      using assms
-      by (metis (full_types) * reborrow_stack.simps(2) reborrow_stack.simps(4)
-          reborrow_stack.simps(6) ref_kind.exhaust)
-  qed
-qed
-
-lemma decomp_reborrow_pop_stack_writable_elims[
-  consumes 4,
-  case_names UniqueUnique SRWUnique SROUnique UniqueSRW SRWSRW SROSRW
-  ]:
-  assumes
-    "writable_stack t stack"
-    "reborrow_pop_stack k t' t stack = stack'"
-    "wf_reborrow stack"
-    "t' \<notin> collect_tags_stack stack"
-    "\<exists>rest. k = Unique \<and> stack' = (Unique, {t'}) # (Unique, {t}) # rest \<Longrightarrow> P"
-    "\<exists>rest. k = SharedReadWrite \<and> stack' = (SharedReadWrite, {t'}) # (Unique, {t}) # rest \<Longrightarrow> P"
-    "\<exists>rest. k = SharedReadOnly \<and> stack' = (SharedReadOnly, {t'}) # (Unique, {t}) # rest \<Longrightarrow> P"
-    "\<exists>rest ts. k = Unique \<and> stack' = (Unique, {t'}) # (SharedReadWrite, ts) # rest \<and> t \<in> ts \<Longrightarrow> P"
-    "\<exists>rest ts. k = SharedReadWrite \<and> stack' = (SharedReadWrite, insert t' ts) # rest \<and> t \<in> ts \<Longrightarrow> P"
-    "\<exists>rest ts. k = SharedReadOnly \<and> stack' = (SharedReadOnly, {t'}) # (SharedReadWrite, ts) # rest \<and> t \<in> ts \<Longrightarrow> P"
-  shows "P"
-  using decomp_reborrow_pop_stack_writable assms by blast
-
-lemma writable_stack_reborrow_pop_stack:
-  assumes
-    "writable_stack t stack"
-    "reborrow_pop_stack k t' t stack = stack'"
-    "wf_reborrow stack"
-    "t' \<notin> collect_tags_stack stack"
-  shows "writable_stack t stack'"
-using assms proof (cases rule: decomp_reborrow_pop_stack_writable_elims)
-  case SROUnique
-  then show ?thesis using assms writable_stack_in_collect_tags by fastforce
-next
-  case SROSRW
-  then show ?thesis using assms writable_stack_in_collect_tags by fastforce
-qed auto
-
-lemma writable_stack_reborrow_pop_stack_derived:
-  assumes
-    "writable_stack t stack"
-    "reborrow_pop_stack k t' t stack = stack'"
-    "wf_reborrow stack"
-    "t' \<notin> collect_tags_stack stack"
-    "k = Unique \<or> k = SharedReadWrite"
-  shows "writable_stack t' stack'"
-using assms proof (cases rule: decomp_reborrow_pop_stack_writable_elims)
-qed auto
+  using reborrow_update_heap' by (metis snd_conv)
 
 lemma reborrow_writable: "\<lbrakk>wf_heap s; writable r s; reborrow k r s = (r', s')\<rbrakk> \<Longrightarrow> writable r s'"
   apply (erule reborrow_elims)
-  apply (simp add: Let_def del: reborrow_pop_stack.simps)
-  apply (rule writable_stack_reborrow_pop_stack)
+  apply (simp add: Let_def del: BorrowStack.reborrow_pop.simps)
+  apply (rule writable_reborrow_pop)
      apply blast
     apply blast
   using wf_tags_spec nth_mem apply blast
@@ -1227,8 +367,8 @@ lemma reborrow_writable_derived:
     "k = Unique \<or> k = SharedReadWrite"
   shows "writable r' s'"
   using assms(3) apply (rule reborrow_elims)
-  using assms apply (simp add: Let_def del: reborrow_pop_stack.simps)
-  apply (rule writable_stack_reborrow_pop_stack_derived[of "tag r" "tags s ! the_ptr (pointer r)" k])
+  using assms apply (simp add: Let_def del: BorrowStack.reborrow_pop.simps)
+  apply (rule writable_reborrow_pop_derived[of "tag r" "tags s ! the_ptr (pointer r)" k])
   using wf_tags_spec apply auto[3]
   using new_tag_notin_at by auto
 
