Rustv/BorrowStack.thy
@@ -1,0 +1,870 @@
+theory BorrowStack
+  imports Defs
+begin
+
+fun collect_tags :: "(ref_kind * tag set) stack \<Rightarrow> tag set" where
+  "collect_tags stack = \<Union>(set (map snd stack))"
+lemma collect_tags_spec:
+  "t \<in> collect_tags stack \<longleftrightarrow> (\<exists>entry \<in> set stack. t \<in> snd entry)"
+proof (induction stack)
+qed auto
+
+inductive wf_reborrow :: "(ref_kind * tag set) stack \<Rightarrow> bool" where
+  (* An allocation root is a Unique reference (Box) *)
+  BorrowRoot: "wf_reborrow [(Unique, {t})]" |
+
+  (* Reborrowing from a Unique reference *)
+  ReborrowUniqueUnique:
+    "\<lbrakk>wf_reborrow ((Unique, {t}) # tail); t' \<notin> insert t (collect_tags tail)\<rbrakk>
+ \<Longrightarrow> wf_reborrow ((Unique, {t'}) # (Unique, {t}) # tail)" |
+  ReborrowUniqueSRW:
+    "\<lbrakk>wf_reborrow ((Unique, {t}) # tail); t' \<notin> insert t (collect_tags tail)\<rbrakk>
+ \<Longrightarrow> wf_reborrow ((SharedReadWrite, {t'}) # (Unique, {t}) # tail)" |
+  ReborrowUniqueSRO:
+    "\<lbrakk>wf_reborrow ((Unique, {t}) # tail); t' \<notin> insert t (collect_tags tail)\<rbrakk>
+ \<Longrightarrow> wf_reborrow ((SharedReadOnly, {t'}) # (Unique, {t}) # tail)" |
+
+  (* Reborrowing from a SharedReadWrite *)
+  ReborrowSRWUnique:
+    "\<lbrakk>wf_reborrow ((SharedReadWrite, ts) # tail); t' \<notin> ts \<union> collect_tags tail\<rbrakk>
+ \<Longrightarrow> wf_reborrow ((Unique, {t'}) # (SharedReadWrite, ts) # tail)" |
+  ReborrowSRWSRW:
+    "\<lbrakk>wf_reborrow ((SharedReadWrite, ts) # tail); t \<notin> ts \<union> collect_tags tail\<rbrakk>
+ \<Longrightarrow> wf_reborrow ((SharedReadWrite, insert t ts) # tail)" |
+  ReborrowSRWSRO:
+    "\<lbrakk>wf_reborrow ((SharedReadWrite, ts) # tail); t' \<notin> ts \<union> collect_tags tail\<rbrakk>
+ \<Longrightarrow> wf_reborrow ((SharedReadOnly, {t'}) # (SharedReadWrite, ts) # tail)" |
+
+  (* Reborrowing from a SharedReadOnly gives only a shared reference *)
+  ReborrowSROSRO:
+    "\<lbrakk>wf_reborrow ((SharedReadOnly, ts) # tail); t \<notin> ts \<union> collect_tags tail\<rbrakk>
+ \<Longrightarrow> wf_reborrow ((SharedReadOnly, insert t ts) # tail)"
+
+inductive_cases wf_reborrow_elims: "wf_reborrow stack"
+
+lemma wf_reborrow_nonempty:
+  assumes "wf_reborrow stack"
+  shows "stack \<noteq> []"
+using assms proof (rule wf_reborrow_elims)
+qed auto
+
+lemma wf_reborrow_root: "wf_reborrow stack \<Longrightarrow> \<exists>t. last stack = (Unique, {t})"
+proof (induction rule: wf_reborrow.induct)
+qed auto
+
+lemma unique_ref_head:
+  assumes "wf_reborrow ((Unique, ts) # end)"
+  shows "\<exists>t. ts = {t}"
+using assms proof (rule wf_reborrow_elims)
+qed auto
+
+lemma unique_ref:
+  assumes
+    "wf_reborrow stack"
+    "(Unique, ts) \<in> set stack"
+  shows "\<exists>t. ts = {t}"
+using assms(1) assms(2) proof (induction rule: wf_reborrow.induct)
+qed auto
+
+lemma wf_reborrow_pop:
+  assumes
+    "wf_reborrow stack"
+    "stack = st1 # st2 # rest"
+  shows "wf_reborrow (st2 # rest)"
+using assms proof (induction arbitrary: st1 rule: wf_reborrow.induct)
+qed auto
+
+lemma wf_reborrow_pop':
+  fixes top rest
+  assumes
+    "wf_reborrow (top # rest)"
+    "rest \<noteq> []"
+  shows "wf_reborrow rest"
+using assms proof (induction "(top # rest)" arbitrary: top rule: wf_reborrow.induct)
+qed auto
+
+lemma shared_read_only_top:
+  assumes
+    "wf_reborrow stack"
+    "\<exists>entry \<in> set stack. fst entry = SharedReadOnly"
+  shows "fst (hd stack) = SharedReadOnly \<and> \<not>(\<exists>entry \<in> set (tl stack). fst entry = SharedReadOnly)"
+using assms proof (induction stack rule: wf_reborrow.induct)
+qed auto
+
+lemma wf_reborrow_top_tag_notin:
+  assumes
+    "wf_reborrow stack"
+    "target \<in> snd (hd stack)"
+  shows "target \<notin> collect_tags (tl stack)"
+using assms proof (induction stack rule: wf_reborrow.induct)
+qed auto
+
+lemma wf_reborrow_tag_position_inj_zero:
+  assumes
+    "wf_reborrow stack"
+    "i < length stack"
+    "target \<in> snd (stack ! i)"
+    "target \<in> snd (stack ! 0)"
+  shows "i = 0"
+proof (cases i)
+  case 0
+  then show ?thesis by simp
+next
+  case (Suc i')
+  have "target \<in> snd (hd stack)" using assms wf_reborrow_nonempty
+    by (simp add: hd_conv_nth)
+  moreover have "target \<in> collect_tags (tl stack)"
+    using assms collect_tags_spec nth_tl wf_reborrow_nonempty
+    by (metis Nitpick.size_list_simp(2) Suc Suc_less_SucD nth_mem)
+  ultimately show ?thesis using wf_reborrow_top_tag_notin assms(1) by blast
+qed
+
+(* repetitive, obvious proof *)
+lemma wf_reborrow_tag_position_inj:
+  assumes
+    "wf_reborrow stack"
+    "i < length stack"
+    "j < length stack"
+    "target \<in> snd (stack ! i)"
+    "target \<in> snd (stack ! j)"
+  shows "i = j"
+using assms proof (induction stack arbitrary: i j rule: wf_reborrow.induct)
+  case (BorrowRoot t)
+  then show ?case by simp
+next
+  case (ReborrowUniqueUnique t tail t')
+  show ?case
+  proof (cases i)
+    case 0
+    then show ?thesis
+      using ReborrowUniqueUnique wf_reborrow.ReborrowUniqueUnique
+        wf_reborrow_tag_position_inj_zero by blast
+  next
+    case (Suc i')
+    note Suci = Suc
+    then show ?thesis
+    proof (cases j)
+      case 0
+      then show ?thesis
+        using ReborrowUniqueUnique wf_reborrow.ReborrowUniqueUnique
+          wf_reborrow_tag_position_inj_zero by blast
+    next
+      case (Suc j')
+      then show ?thesis using Suc Suci ReborrowUniqueUnique by auto
+    qed
+  qed
+next
+  case (ReborrowUniqueSRW t tail t')
+  then show ?case
+  proof (cases i)
+    case 0
+    then show ?thesis
+      using ReborrowUniqueSRW wf_reborrow.ReborrowUniqueSRW
+        wf_reborrow_tag_position_inj_zero by blast
+  next
+    case (Suc i')
+    note Suci = Suc
+    then show ?thesis
+    proof (cases j)
+      case 0
+      then show ?thesis
+        using ReborrowUniqueSRW wf_reborrow.ReborrowUniqueSRW
+          wf_reborrow_tag_position_inj_zero by blast
+    next
+      case (Suc j')
+      then show ?thesis using Suc Suci ReborrowUniqueSRW by auto
+    qed
+  qed
+next
+  case (ReborrowUniqueSRO t tail t')
+  then show ?case
+  proof (cases i)
+    case 0
+    then show ?thesis
+      using ReborrowUniqueSRO wf_reborrow.ReborrowUniqueSRO
+        wf_reborrow_tag_position_inj_zero by blast
+  next
+    case (Suc i')
+    note Suci = Suc
+    then show ?thesis
+    proof (cases j)
+      case 0
+      then show ?thesis
+      using ReborrowUniqueSRO wf_reborrow.ReborrowUniqueSRO
+        wf_reborrow_tag_position_inj_zero by blast
+    next
+      case (Suc j')
+      then show ?thesis using Suc Suci ReborrowUniqueSRO by auto
+    qed
+  qed
+next
+  case (ReborrowSRWUnique ts tail t')
+  then show ?case
+  proof (cases i)
+    case 0
+    then show ?thesis
+      using ReborrowSRWUnique wf_reborrow.ReborrowSRWUnique
+        wf_reborrow_tag_position_inj_zero by blast
+  next
+    case (Suc i')
+    note Suci = Suc
+    then show ?thesis
+    proof (cases j)
+      case 0
+      then show ?thesis
+      using ReborrowSRWUnique wf_reborrow.ReborrowSRWUnique
+        wf_reborrow_tag_position_inj_zero by blast
+    next
+      case (Suc j')
+      then show ?thesis using Suc Suci ReborrowSRWUnique by auto
+    qed
+  qed
+next
+  case (ReborrowSRWSRW ts tail t)
+  then show ?case
+  proof (cases i)
+    case 0
+    then show ?thesis
+      using ReborrowSRWSRW wf_reborrow.ReborrowSRWSRW
+        wf_reborrow_tag_position_inj_zero by blast
+  next
+    case (Suc i')
+    note Suci = Suc
+    then show ?thesis
+    proof (cases j)
+      case 0
+      then show ?thesis
+      using ReborrowSRWSRW wf_reborrow.ReborrowSRWSRW
+        wf_reborrow_tag_position_inj_zero by blast
+    next
+      case (Suc j')
+      then show ?thesis using Suc Suci ReborrowSRWSRW
+        by (metis length_Cons nth_Cons_Suc)
+    qed
+  qed
+next
+  case (ReborrowSRWSRO ts tail t')
+  then show ?case
+  proof (cases i)
+    case 0
+    then show ?thesis
+      using ReborrowSRWSRO wf_reborrow.ReborrowSRWSRO
+        wf_reborrow_tag_position_inj_zero by blast
+  next
+    case (Suc i')
+    note Suci = Suc
+    then show ?thesis
+    proof (cases j)
+      case 0
+      then show ?thesis
+      using ReborrowSRWSRO wf_reborrow.ReborrowSRWSRO
+        wf_reborrow_tag_position_inj_zero by blast
+    next
+      case (Suc j')
+      then show ?thesis using Suc Suci ReborrowSRWSRO by auto
+    qed
+  qed
+next
+  case (ReborrowSROSRO ts tail t)
+  then show ?case
+  proof (cases i)
+    case 0
+    then show ?thesis
+      using ReborrowSROSRO wf_reborrow.ReborrowSROSRO
+        wf_reborrow_tag_position_inj_zero by blast
+  next
+    case (Suc i')
+    note Suci = Suc
+    then show ?thesis
+    proof (cases j)
+      case 0
+      then show ?thesis
+      using ReborrowSROSRO wf_reborrow.ReborrowSROSRO
+        wf_reborrow_tag_position_inj_zero by blast
+    next
+      case (Suc j')
+      then show ?thesis using Suc Suci ReborrowSROSRO
+        by (metis length_Cons nth_Cons_Suc)
+    qed
+  qed
+qed
+
+lemma wf_reborrow_tag_position_unique':
+  assumes
+    "wf_reborrow stack"
+    "target \<in> collect_tags stack"
+  shows "\<exists>i. (i < length stack \<and> target \<in> snd (stack ! i)) \<and>
+  (\<forall>j. j < length stack \<and> target \<in> snd (stack ! j) \<longrightarrow> j = i)"
+proof -
+  have "\<exists>i < length stack. target \<in> snd (stack ! i)"
+    using assms collect_tags_spec by (metis in_set_conv_nth)
+  then obtain i where
+    "i < length stack"
+    "target \<in> snd (stack ! i)"
+    by auto
+  moreover
+  note calc = calculation
+  have "\<forall>j. j < length stack \<and> target \<in> snd (stack ! j) \<longrightarrow> j = i"
+  proof
+    fix j
+    show "j < length stack \<and> target \<in> snd (stack ! j) \<longrightarrow> j = i"
+    proof
+      assume "j < length stack \<and> target \<in> snd (stack ! j)"
+      then show "j = i" using calc assms wf_reborrow_tag_position_inj by auto
+    qed
+  qed
+  ultimately show "\<exists>i. (i < length stack \<and> target \<in> snd (stack ! i)) \<and>
+    (\<forall>j. j < length stack \<and> target \<in> snd (stack ! j) \<longrightarrow> j = i)"
+    by blast
+qed
+
+lemma wf_reborrow_tag_position_unique:
+  assumes
+    "wf_reborrow stack"
+    "target \<in> collect_tags stack"
+  shows "\<exists>!i. i < length stack \<and> target \<in> snd (stack ! i)"
+  using wf_reborrow_tag_position_unique' assms by blast
+
+fun stack_finite :: "(ref_kind * tag set) stack \<Rightarrow> bool" where
+  "stack_finite [] = True" |
+  "stack_finite (s # stack) = (finite (snd s) \<and> stack_finite stack)"
+
+lemma stack_finite_spec: "stack_finite stack \<longleftrightarrow> (\<forall>s \<in> set stack. finite (snd s))"
+proof (induction stack)
+qed auto
+
+lemma collect_tags_stack_finite:
+  assumes "stack_finite stack"
+  shows "finite (collect_tags stack)"
+  using assms stack_finite_spec by auto
+
+lemma stack_finite_finite_collect_tags:
+  assumes "finite (collect_tags stack)"
+  shows "stack_finite stack"
+  using assms by (simp add: stack_finite_spec)
+
+fun pop_tags :: "tag \<Rightarrow> (ref_kind * tag set) stack \<Rightarrow> (ref_kind * tag set) stack" where
+  "pop_tags t stack = dropWhile (\<lambda>entry. t \<notin> snd entry) stack"
+
+lemma hd_dropWhile_stack:
+  assumes
+    "pop_tags t stack = stack'"
+    "\<exists>entry \<in> set stack. t \<in> snd entry"
+  shows "t \<in> snd (hd stack')"
+  by (metis assms(1) assms(2) pop_tags.simps dropWhile_eq_Nil_conv hd_dropWhile)
+
+lemma dropWhile_stack_reborrow:
+  "wf_reborrow stack \<and> dropWhile P stack \<noteq> [] \<Longrightarrow> wf_reborrow (dropWhile P stack)"
+proof (induction stack)
+  case Nil
+  then show ?case using wf_reborrow_nonempty by simp
+next
+  case (Cons top rest)
+  show ?case
+  proof (cases "P top")
+    case True
+    moreover have "dropWhile P rest \<noteq> []" using Cons.prems calculation by auto
+    moreover have "rest \<noteq> []" using calculation by auto
+    moreover have "wf_reborrow rest" using calculation Cons.prems wf_reborrow_pop' by auto
+    ultimately show ?thesis using Cons.IH by auto
+  next
+    case False
+    then show ?thesis using Cons.prems by simp
+  qed
+qed
+
+lemma dropWhile_stack_finite:
+  "stack_finite stack \<Longrightarrow> stack_finite (dropWhile P stack)"
+proof (induction stack)
+  case Nil
+  then show ?case by simp
+next
+  case (Cons st stack)
+  then have *: "stack_finite (dropWhile P stack)" by simp
+  then show ?case
+  proof (cases "P st")
+    case True
+    then show ?thesis using * by simp
+  next
+    case False
+    then show ?thesis using Cons.prems by simp
+  qed
+qed
+
+fun writable :: "tag \<Rightarrow> (ref_kind * tag set) stack \<Rightarrow> bool" where
+  "writable t [] \<longleftrightarrow> False" |
+  "writable t ((k, ts) # stack) \<longleftrightarrow>
+    (if t \<in> ts then k = Unique \<or> k = SharedReadWrite else writable t stack)"
+
+lemma writable_in_collect_tags:
+  assumes "writable t stack"
+  shows "t \<in> collect_tags stack"
+using assms proof (induction stack)
+  case (Cons entry stack)
+  then show ?case using writable.elims(2) by fastforce
+qed auto
+
+lemma writable_the_index:
+  assumes
+    "wf_reborrow stack"
+    "writable t stack"
+  shows "\<exists>!i. i < length stack \<and> t \<in> snd (stack ! i)"
+  using wf_reborrow_tag_position_unique writable_in_collect_tags assms by simp
+
+lemma writable_pop_tags:
+  "writable t stack \<Longrightarrow> writable t (pop_tags t stack)"
+proof (induction stack)
+  case Nil
+  then show ?case by simp
+next
+  case (Cons entry stack)
+  then show ?case using writable.elims(2) by fastforce
+qed
+
+lemma writable_pop_tags':
+  assumes
+    "writable t stack"
+    "pop_tags t stack = stack'"
+  shows "(fst (hd stack') = Unique \<or> fst (hd stack') = SharedReadWrite)
+      \<and> t \<in> snd (hd stack')"
+    (is "?kind \<and> _")
+proof
+  show ?kind
+    using assms
+    by (metis hd_dropWhile list.collapse pop_tags.elims prod.collapse writable.simps(1)
+        writable.simps(2) writable_pop_tags)
+next
+  show "t \<in> snd (hd stack')"
+    using hd_dropWhile_stack assms writable_in_collect_tags by simp
+qed
+
+fun reborrow :: "ref_kind \<Rightarrow> tag \<Rightarrow> (ref_kind * tag set) stack \<Rightarrow> (ref_kind * tag set) stack"
+  where
+  (* reborrwing Unique *)
+  "reborrow Unique t ((Unique, ts) # stack) = (Unique, {t}) # (Unique, ts) # stack" |
+  "reborrow Unique t ((SharedReadWrite, ts) # stack) =
+    (Unique, {t}) # (SharedReadWrite, ts) # stack" |
+  (* reborrowing SharedReadWrite *)
+  "reborrow SharedReadWrite t ((Unique, ts) # stack) =
+    (SharedReadWrite, {t}) # (Unique, ts) # stack" |
+  "reborrow SharedReadWrite t ((SharedReadWrite, ts) # stack) =
+    (SharedReadWrite, insert t ts) # stack" |
+  (* reborrwing SharedReadOnly *)
+  "reborrow SharedReadOnly t ((Unique, ts) # stack) =
+    (SharedReadOnly, {t}) # (Unique, ts) # stack" |
+  "reborrow SharedReadOnly t ((SharedReadWrite, ts) # stack) =
+    (SharedReadOnly, {t}) # (SharedReadWrite, ts) # stack" |
+  "reborrow SharedReadOnly t ((SharedReadOnly, ts) # stack) =
+    (SharedReadOnly, insert t ts) # stack" |
+  (* other cases are uninteresting as reborrow is not well-formed *)
+  "reborrow _ _ [] = []" |
+  "reborrow Unique _ ((SharedReadOnly, _) # stack) = []" |
+  "reborrow SharedReadWrite _ ((SharedReadOnly, _) # stack) = []"
+
+lemma reborrow_hd:
+  assumes
+    "reborrow r t stack = stack'"
+    "stack' \<noteq> []"
+  shows "r = fst (hd stack') \<and> t \<in> snd (hd stack')"
+using assms proof (cases rule: reborrow.elims)
+qed auto
+
+fun_cases reborrow_elims_Unique[case_names _ UniqueUnique UniqueSRW]:
+  "reborrow Unique t stack = (Unique, ts) # stack'"
+fun_cases reborrow_elims_SRW[case_names _ SRWUnique SRWSRW]:
+  "reborrow SharedReadWrite t stack = (SharedReadWrite, ts) # stack'"
+fun_cases reborrow_elims_SRO[case_names _ SROUnique SROSRW SROSRO]:
+  "reborrow SharedReadOnly t stack = (SharedReadOnly, ts) # stack'"
+
+lemma wf_reborrow_reborrow_Unique:
+  assumes
+    "wf_reborrow stack"
+    "t \<notin> collect_tags stack"
+    "reborrow Unique t stack = stack'"
+    "stack' \<noteq> []"
+  shows "wf_reborrow stack'"
+proof -
+  have p: "Unique = fst (hd stack') \<and> t \<in> snd (hd stack')"
+    using assms reborrow_hd by simp
+  then obtain ts rest where
+    q: "stack' = (Unique, ts) # rest"
+    using assms by (metis list.collapse prod.collapse)
+  then have "wf_reborrow ((Unique, ts) # rest)"
+  proof (cases t stack ts rest rule: reborrow_elims_Unique)
+    case _
+    then show ?case using assms(3) q by blast
+  next
+    case (UniqueUnique ts' stack)
+    moreover obtain t' where
+      "ts' = {t'}"
+      using assms(1) calculation(1) unique_ref_head by blast
+    moreover have "wf_reborrow ((Unique, {t}) # (Unique, {t'}) # stack)"
+    proof (rule ReborrowUniqueUnique)
+      show "wf_reborrow ((Unique, {t'}) # stack)"
+        using assms(1) calculation(1) calculation(4) by auto
+    next
+      have "t \<notin> {t'} \<union> collect_tags stack"
+        using assms(2) calculation(1) calculation(4) by auto
+      then show "t \<notin> insert t' (collect_tags stack)" by simp
+    qed
+    ultimately show ?thesis by simp
+  next
+    case (UniqueSRW ts' stack)
+    moreover have "wf_reborrow ((Unique, {t}) # (SharedReadWrite, ts') # stack)"
+    proof (rule ReborrowSRWUnique)
+      show "wf_reborrow ((SharedReadWrite, ts') # stack)"
+        using assms(1) calculation(1) by blast
+    next
+      show "t \<notin> ts' \<union> collect_tags stack"
+        using assms(2) calculation(1) by auto
+    qed
+    ultimately show ?thesis by simp
+  qed
+  then show ?thesis by (simp add: q)
+qed
+
+lemma wf_reborrow_reborrow_SRW:
+  assumes
+    "wf_reborrow stack"
+    "t \<notin> collect_tags stack"
+    "reborrow SharedReadWrite t stack = stack'"
+    "stack' \<noteq> []"
+  shows "wf_reborrow stack'"
+proof -
+  have p: "SharedReadWrite = fst (hd stack') \<and> t \<in> snd (hd stack')"
+    using assms reborrow_hd by simp
+  then obtain ts rest where
+    q: "stack' = (SharedReadWrite, ts) # rest"
+    using assms by (metis list.collapse prod.collapse)
+  then have "wf_reborrow ((SharedReadWrite, ts) # rest)"
+  proof (cases t stack ts rest rule: reborrow_elims_SRW)
+    case _
+    then show ?case using assms(3) q by blast
+  next
+    case (SRWUnique ts' stack)
+    moreover obtain t' where
+      "ts' = {t'}"
+      using assms(1) calculation(1) unique_ref_head by blast
+    moreover have "wf_reborrow ((SharedReadWrite, {t}) # (Unique, {t'}) # stack)"
+    proof (rule ReborrowUniqueSRW)
+      show "wf_reborrow ((Unique, {t'}) # stack)"
+        using assms SRWUnique calculation by simp
+    next
+      have "t \<notin> {t'} \<union> (collect_tags stack)"
+        using assms(2) calculation(1) calculation(4) by auto
+      then show "t \<notin> insert t' (collect_tags stack)" by auto
+    qed
+    moreover have "wf_reborrow ((SharedReadWrite, ts) # (Unique, ts') # stack)"
+      using calculation by simp
+    ultimately show ?thesis by simp
+  next
+    case (SRWSRW ts')
+    moreover have "wf_reborrow ((SharedReadWrite, insert t ts') # rest)"
+    proof (rule ReborrowSRWSRW)
+      show "wf_reborrow ((SharedReadWrite, ts') # rest)" using assms SRWSRW by simp
+    next
+      show "t \<notin> ts' \<union> collect_tags rest" using assms SRWSRW by simp
+    qed
+    ultimately show ?thesis by simp
+  qed
+  then show ?thesis by (simp add: q)
+qed
+
+lemma wf_reborrow_reborrow_SRO:
+  assumes
+    "wf_reborrow stack"
+    "t \<notin> collect_tags stack"
+    "reborrow SharedReadOnly t stack = stack'"
+    "stack' \<noteq> []"
+  shows "wf_reborrow stack'"
+proof -
+  have p: "SharedReadOnly = fst (hd stack') \<and> t \<in> snd (hd stack')"
+    using assms reborrow_hd by simp
+  then obtain ts rest where
+    q: "stack' = (SharedReadOnly, ts) # rest"
+    using assms by (metis list.collapse prod.collapse)
+  then have "wf_reborrow ((SharedReadOnly, ts) # rest)"
+  proof (cases t stack ts rest rule: reborrow_elims_SRO)
+    case _
+    then show ?case using assms(3) q by blast
+  next
+    case (SROUnique ts' stack)
+    moreover obtain t' where
+      "ts' = {t'}"
+      using assms(1) calculation(1) unique_ref_head by blast
+    moreover have "wf_reborrow ((SharedReadOnly, {t}) # (Unique, {t'}) # stack)"
+    proof (rule ReborrowUniqueSRO)
+      show "wf_reborrow ((Unique, {t'}) # stack)"
+        using assms calculation by simp
+    next
+      have "t \<notin> {t'} \<union> collect_tags stack"
+        using assms(2) calculation(1) calculation(4) by auto
+      then show "t \<notin> insert t' (collect_tags stack)" by simp
+    qed
+    ultimately show ?thesis by (simp add: q)
+  next
+    case (SROSRW ts' stack)
+    moreover have "wf_reborrow ((SharedReadOnly, {t}) # (SharedReadWrite, ts') # stack)"
+    proof (rule ReborrowSRWSRO)
+      show "wf_reborrow ((SharedReadWrite, ts') # stack)"
+        using assms(1) calculation(1) by auto
+    next
+      show "t \<notin> ts' \<union> collect_tags stack"
+        using assms(2) calculation(1) by fastforce
+    qed
+    ultimately show ?thesis by (simp add: q)
+  next
+    case (SROSRO ts')
+    moreover have "wf_reborrow ((SharedReadOnly, insert t ts') # rest)"
+    proof (rule ReborrowSROSRO)
+      show "wf_reborrow ((SharedReadOnly, ts') # rest)"
+        using assms(1) calculation(1) by blast
+    next
+      show "t \<notin> ts' \<union> collect_tags rest" using assms SROSRO by simp
+    qed
+    ultimately show ?thesis by simp
+  qed
+  then show ?thesis by (simp add: q)
+qed
+
+lemma wf_reborrow_reborrow:
+  assumes
+    "wf_reborrow stack"
+    "t \<notin> collect_tags stack"
+    "reborrow k t stack = stack'"
+    "stack' \<noteq> []"
+  shows "wf_reborrow stack'"
+proof (cases k)
+  case Unique
+  then show ?thesis using assms wf_reborrow_reborrow_Unique by simp
+next
+  case SharedReadWrite
+  then show ?thesis using assms wf_reborrow_reborrow_SRW by simp
+next
+  case SharedReadOnly
+  then show ?thesis using assms wf_reborrow_reborrow_SRO by simp
+qed
+
+lemma collect_tags_reborrow_subset:
+  assumes "reborrow k t stack = stack'"
+  shows "collect_tags stack' \<subseteq> {t} \<union> collect_tags stack"
+using assms proof(cases rule: reborrow.elims)
+qed auto
+
+lemma stack_finite_reborrow:
+  assumes
+    "reborrow k t stack = stack'"
+    "stack_finite stack"
+  shows "stack_finite stack'"
+using assms collect_tags_reborrow_subset stack_finite_finite_collect_tags
+  by (meson collect_tags_stack_finite finite.emptyI finite.insertI finite_Un finite_subset)
+
+lemma notin_pop_tags:
+  assumes "pop_tags t stack = stack'"
+  shows "collect_tags stack' \<subseteq> collect_tags stack"
+using assms proof (induction stack arbitrary: stack')
+  case Nil
+  then show ?case by simp
+next
+  case (Cons entry stack)
+  show ?case
+  proof (cases "t \<in> snd entry")
+    case True
+    then have "stack' = entry # stack" using Cons.prems by simp
+    then show ?thesis by simp
+  next
+    case False
+    then have "stack' = pop_tags t stack" using Cons.prems by simp
+    then show ?thesis using Cons.IH by auto
+  qed
+qed
+
+lemma wf_reborrow_reborrow_pop:
+  assumes
+    "wf_reborrow stack"
+    "writable old stack"
+    "pop_tags old stack = popped"
+    "reborrow k new popped = stack'"
+    "new \<notin> collect_tags stack"
+  shows "wf_reborrow stack'"
+proof -
+  have p: "wf_reborrow popped"
+    using assms
+    by (metis dropWhile_stack_reborrow BorrowStack.pop_tags.elims
+        writable.simps(1) writable_pop_tags)
+  have q: "new \<notin> collect_tags popped"
+    using assms notin_pop_tags by fastforce
+  have "(fst (hd popped) = Unique \<and> old \<in> snd (hd popped))
+      \<or> (fst (hd popped) = SharedReadWrite \<and> old \<in> snd (hd popped))"
+    using assms writable_pop_tags' by blast
+  then show ?thesis
+  proof
+    assume "fst (hd popped) = Unique \<and> old \<in> snd (hd popped)"
+    then obtain ts rest where
+      "popped = (Unique, ts) # rest"
+      "old \<in> ts"
+      by (metis assms(2) assms(3) list.collapse prod.collapse
+          writable.simps(1) writable_pop_tags)
+    moreover have "ts = {old}" using calculation assms p unique_ref_head by fastforce
+    moreover have "reborrow k new ((Unique, {old}) # rest) = stack'"
+      using assms calculation by simp
+    then show ?thesis
+    proof (rule reborrow.elims, auto)
+      show "wf_reborrow ((Unique, {new}) # (Unique, {old}) # rest)"
+        using assms calculation p q ReborrowUniqueUnique by simp
+    next
+      show "wf_reborrow ((SharedReadWrite, {new}) # (Unique, {old}) # rest)"
+        using assms calculation p q ReborrowUniqueSRW by simp
+    next
+      show "wf_reborrow ((SharedReadOnly, {new}) # (Unique, {old}) # rest)"
+        using assms calculation p q ReborrowUniqueSRO by simp
+    qed
+  next
+    assume "fst (hd popped) = SharedReadWrite \<and> old \<in> snd (hd popped)"
+    then obtain ts rest where
+      "popped = (SharedReadWrite, ts) # rest"
+      "old \<in> ts"
+      by (metis assms(2) assms(3) list.collapse prod.collapse
+          writable.simps(1) writable_pop_tags)
+    moreover have "reborrow k new ((SharedReadWrite, ts) # rest) = stack'"
+      using assms calculation by simp
+    then show ?thesis
+    proof (rule reborrow.elims, auto)
+      show "wf_reborrow ((Unique, {new}) # (SharedReadWrite, ts) # rest)"
+        using assms calculation p q ReborrowSRWUnique by simp
+    next
+      show "wf_reborrow ((SharedReadWrite, insert new ts) # rest)"
+        using assms calculation p q ReborrowSRWSRW by simp
+    next
+      show "wf_reborrow ((SharedReadOnly, {new}) # (SharedReadWrite, ts) # rest)"
+        using assms calculation p q ReborrowSRWSRO by simp
+    qed
+  qed
+qed
+
+fun reborrow_pop :: "ref_kind \<Rightarrow> tag \<Rightarrow> tag \<Rightarrow> (ref_kind * tag set) stack \<Rightarrow> (ref_kind * tag set) stack" where
+  "reborrow_pop k child parent stack =
+    reborrow k child (pop_tags parent stack)"
+
+lemma reborrow_pop_subset:
+  "collect_tags (reborrow_pop k child parent stack) \<subseteq> {child} \<union> collect_tags stack"
+proof (induction stack arbitrary: child parent)
+  case Nil
+  then show ?case by simp
+next
+  case (Cons entry stack)
+  then show ?case
+    by (metis collect_tags_reborrow_subset insert_is_Un insert_mono
+        notin_pop_tags reborrow_pop.elims subset_trans)
+qed
+
+lemma decomp_pop_tags_writable:
+  assumes
+    "writable t stack"
+    "pop_tags t stack = stack'"
+    "wf_reborrow stack"
+  shows "(\<exists>rest. stack' = (Unique, {t}) # rest)
+  \<or> (\<exists>rest ts. stack' = (SharedReadWrite, ts) # rest \<and> t \<in> ts)"
+using assms proof (induction stack)
+  case Nil
+  then show ?case by simp
+next
+  case (Cons entry stack)
+  then show ?case
+  proof (cases "t \<in> snd entry")
+    case True
+    moreover have "stack' = entry # stack" using Cons.prems calculation by simp
+    moreover have "fst entry = Unique \<or> fst entry = SharedReadWrite"
+      using Cons.prems(1) Cons.prems(2) calculation(2) writable_pop_tags' by fastforce
+    moreover have "entry = (Unique, {t}) \<or> (\<exists>ts. entry = (SharedReadWrite, ts) \<and> t \<in> ts)"
+      using Cons calculation
+      by (metis empty_iff insert_iff prod.collapse unique_ref_head)
+    ultimately show ?thesis by simp
+  next
+    case False
+    moreover have "writable t stack" using Cons.prems calculation
+      by (metis eq_snd_iff list.inject writable.elims(2))
+    moreover have "pop_tags t stack = stack'" using Cons.prems calculation by simp
+    moreover have "wf_reborrow stack"
+      using Cons.prems wf_reborrow_pop' calculation(2) writable.simps(1) by blast
+    ultimately show ?thesis using Cons.IH by simp
+  qed
+qed
+
+lemma decomp_reborrow_pop_writable:
+  assumes
+    "writable t stack"
+    "reborrow_pop k t' t stack = stack'"
+    "wf_reborrow stack"
+  shows "
+  (\<exists>rest. k = Unique \<and> stack' = (Unique, {t'}) # (Unique, {t}) # rest)
+  \<or> (\<exists>rest. k = SharedReadWrite \<and> stack' = (SharedReadWrite, {t'}) # (Unique, {t}) # rest)
+  \<or> (\<exists>rest. k = SharedReadOnly \<and> stack' = (SharedReadOnly, {t'}) # (Unique, {t}) # rest)
+  \<or> (\<exists>rest ts. k = Unique \<and>  stack' = (Unique, {t'}) # (SharedReadWrite, ts) # rest \<and> t \<in> ts)
+  \<or> (\<exists>rest ts. k = SharedReadWrite \<and> stack' = (SharedReadWrite, insert t' ts) # rest \<and> t \<in> ts)
+  \<or> (\<exists>rest ts. k = SharedReadOnly \<and> stack' = (SharedReadOnly, {t'}) # (SharedReadWrite, ts) # rest \<and> t \<in> ts)"
+proof -
+  have *: "reborrow k t' (pop_tags t stack) = stack'" (is "reborrow _ _ ?popped = _")
+    using assms by simp
+  then have "(\<exists>rest. ?popped = (Unique, {t}) # rest)
+  \<or> (\<exists>rest ts. ?popped = (SharedReadWrite, ts) # rest \<and> t \<in> ts)"
+    using assms decomp_pop_tags_writable by simp
+  then show ?thesis
+  proof
+    assume "\<exists>rest. ?popped = (Unique, {t}) # rest"
+    then show ?thesis
+      using assms
+      by (metis (full_types) "*" reborrow.simps(1) reborrow.simps(3)
+          reborrow.simps(5) ref_kind.exhaust)
+  next
+    assume "\<exists>rest ts. ?popped = (SharedReadWrite, ts) # rest \<and> t \<in> ts"
+    then show ?thesis
+      using assms
+      by (metis (full_types) * reborrow.simps(2) reborrow.simps(4)
+          reborrow.simps(6) ref_kind.exhaust)
+  qed
+qed
+
+lemma decomp_reborrow_pop_writable_elims[
+  consumes 3,
+  case_names UniqueUnique SRWUnique SROUnique UniqueSRW SRWSRW SROSRW
+  ]:
+  assumes
+    "writable t stack"
+    "reborrow_pop k t' t stack = stack'"
+    "wf_reborrow stack"
+    "\<exists>rest. k = Unique \<and> stack' = (Unique, {t'}) # (Unique, {t}) # rest \<Longrightarrow> P"
+    "\<exists>rest. k = SharedReadWrite \<and> stack' = (SharedReadWrite, {t'}) # (Unique, {t}) # rest \<Longrightarrow> P"
+    "\<exists>rest. k = SharedReadOnly \<and> stack' = (SharedReadOnly, {t'}) # (Unique, {t}) # rest \<Longrightarrow> P"
+    "\<exists>rest ts. k = Unique \<and> stack' = (Unique, {t'}) # (SharedReadWrite, ts) # rest \<and> t \<in> ts \<Longrightarrow> P"
+    "\<exists>rest ts. k = SharedReadWrite \<and> stack' = (SharedReadWrite, insert t' ts) # rest \<and> t \<in> ts \<Longrightarrow> P"
+    "\<exists>rest ts. k = SharedReadOnly \<and> stack' = (SharedReadOnly, {t'}) # (SharedReadWrite, ts) # rest \<and> t \<in> ts \<Longrightarrow> P"
+  shows "P"
+  using decomp_reborrow_pop_writable assms by blast
+
+lemma writable_reborrow_pop:
+  assumes
+    "writable t stack"
+    "reborrow_pop k t' t stack = stack'"
+    "wf_reborrow stack"
+    "t' \<notin> collect_tags stack"
+  shows "writable t stack'"
+using assms proof (cases rule: decomp_reborrow_pop_writable_elims)
+  case SROUnique
+  then show ?thesis using assms writable_in_collect_tags by fastforce
+next
+  case SROSRW
+  then show ?thesis using assms writable_in_collect_tags by fastforce
+qed auto
+
+lemma writable_reborrow_pop_derived:
+  assumes
+    "writable t stack"
+    "reborrow_pop k t' t stack = stack'"
+    "wf_reborrow stack"
+    "k = Unique \<or> k = SharedReadWrite"
+  shows "writable t' stack'"
+using assms proof (cases rule: decomp_reborrow_pop_writable_elims)
+qed auto
+
+end
