Rustv/Defs.thy
@@ -1,0 +1,23 @@
+theory Defs
+  imports Main
+begin
+
+datatype rust_error = invalid_ref
+
+datatype pointer = ptr_val nat
+datatype tag = tag_val nat
+datatype val = int_val int
+record tagged_ref =
+  pointer :: pointer
+  tag :: tag
+
+fun the_ptr :: "pointer \<Rightarrow> nat" where
+  "the_ptr (ptr_val p) = p"
+
+fun the_tag :: "tag \<Rightarrow> nat" where
+  "the_tag (tag_val t) = t"
+
+datatype ref_kind = Unique | SharedReadWrite | SharedReadOnly
+type_synonym 'a stack = "'a list"
+
+end
